Initial proof of mergesort

coq-osiris/examples/src/merge.ml
@@ -24,3 +24,13 @@ let rec split l =
      let (l1, l2) = split t in
                  x1::l1, x2::l2
 
+let rec merge_sort l =
+  match l with
+  | [] -> []
+  | [x] -> [x]
+  | _ ->
+     let l1, l2 = split l in
+     let l1' = merge_sort l1 in
+     let l2' = merge_sort l2 in
+     merge2 l1' l2'
+
